casestudy/ImpCompCert/zero/Impltl.v
@@ -1,0 +1,15 @@
+
+family Impzero.LTL extends Impbackend {
+    Definition node := positive
+
+    Inductive instruction += 
+      | Lbranch (s: node)
+}
+
+family Impzero.LTL.Semantics {
+  Inductive step : state -> state -> Prop += 
+     | exec_Lbranch: forall s f sp pc bb rs m,
+         step (Block s f sp (Lbranch pc :: bb) rs m)
+              (State s f sp pc rs m)
+}
+
