casestudy/ImpCompCert/zero/Implinear.v
@@ -1,0 +1,11 @@
+
+(* Nothing to do here *)
+family Impzero.Implinear extends Impbackend { }
+
+(* LTL -> Linear translation *)
+family Impzero.Implinearize extends ImpbackendTransform {  
+  family Source extends Impltl { }
+  family Target extends Implinear { }
+
+  family CorrectnessProof { }
+}
