casestudy/ImpCompCert/zero/Imprtl.v
@@ -1,0 +1,3 @@
+
+(* There should be some sharing at least... *)
+family Imzero.Imprtl { }
